RthetaWriterMonad.v
@@ -1,0 +1,126 @@
+
+Require Import Coq.Bool.Bool.
+Require Import Ring.
+
+(* CoRN MathClasses *)
+Require Import MathClasses.interfaces.abstract_algebra.
+Require Import MathClasses.theory.rings.
+Require Import MathClasses.interfaces.orders MathClasses.orders.orders.
+
+Require Import Rtheta.
+
+Require Import CpdtTactics.
+Require Import JRWTactics.
+
+Require Import ExtLib.Core.Type.
+Require Import ExtLib.Structures.Monads.
+Require Import ExtLib.Structures.Monoid.
+Require Import ExtLib.Data.Monads.WriterMonad.
+Require Import ExtLib.Data.Monads.IdentityMonad.
+Require Import WriterMonadNoT.
+Require Import ExtLib.Structures.MonadLaws.
+
+Import MonadNotation.
+Local Open Scope monad_scope.
+
+Definition Monoid_RthetaFlags : Monoid RthetaFlags := Build_Monoid combineFlags RthetaFlags_normal.
+
+Definition flags_m : Type -> Type := writer Monoid_RthetaFlags.
+Context {Writer_flags: MonadWriter Monoid_RthetaFlags flags_m}.
+
+Definition Rtheta_liftM
+           (op: Rtheta -> Rtheta)
+           (xm: flags_m Rtheta) : flags_m Rtheta :=
+  x <- xm ;;
+    tell
+    (let xs := (is_struct x) in
+     (computeFlags xs xs))
+    ;;
+    ret (op x).
+
+Definition Rtheta_liftM2
+           (op: Rtheta -> Rtheta -> Rtheta)
+           (am bm: flags_m Rtheta) : flags_m Rtheta :=
+  a <- am ;;  b <- bm ;;
+    tell (computeFlags (is_struct a) (is_struct b)) ;;
+    ret (op a b).
+
+
+Global Instance Rtheta_Mequiv: Equiv (flags_m Rtheta) :=
+  fun am bm => (evalWriter am) = (evalWriter bm).
+
+Ltac unfold_Rtheta_Mequiv := unfold equiv, Rtheta_Mequiv in *.
+
+Instance Rtheta_MSetoid: Setoid (flags_m Rtheta).
+Proof.
+  split.
+  unfold Reflexive. destruct x; (unfold_Rtheta_Mequiv; crush).
+  unfold Symmetric. intros. destruct x,y; (unfold_Rtheta_Mequiv; crush).
+  unfold Transitive. intros. destruct x,y,z; unfold_Rtheta_Mequiv; crush.
+Qed.
+
+Lemma evalWriter_Rtheta_liftM
+      (op: Rtheta -> Rtheta)
+      {a: flags_m Rtheta}
+  :
+    evalWriter (Rtheta_liftM op a) ≡ op (evalWriter a).
+Proof.
+  reflexivity.
+Qed.
+
+Lemma evalWriter_lift_Rtheta_liftM2
+      (op: Rtheta -> Rtheta -> Rtheta)
+      {a b: flags_m Rtheta}
+  :
+    evalWriter (Rtheta_liftM2 op a b) ≡ op (evalWriter a) (evalWriter b).
+Proof.
+  reflexivity.
+Qed.
+
+Definition Rtheta_evalRel
+           (rel: Rtheta -> Rtheta -> Prop)
+           (am bm: flags_m Rtheta) : Prop :=
+  rel (evalWriter am) (evalWriter bm).
+
+
+Global Instance Rtheta_MZero: Zero (flags_m Rtheta) := ret (Rtheta_normal zero).
+Global Instance Rtheta_MOne: One (flags_m Rtheta) := ret (Rtheta_normal one).
+Global Instance Rtheta_MPlus: Plus (flags_m Rtheta) := Rtheta_liftM2 (Rtheta_binop plus).
+Global Instance Rtheta_MMult: Mult (flags_m Rtheta) := Rtheta_liftM2 (Rtheta_binop mult).
+Global Instance Rtheta_MNeg: Negate (flags_m Rtheta) := Rtheta_liftM (Rtheta_unary negate).
+Global Instance Rtheta_MLe: Le (flags_m Rtheta) := Rtheta_evalRel (Rtheta_rel_first le).
+Global Instance Rtheta_MLt: Lt (flags_m Rtheta) := Rtheta_evalRel (Rtheta_rel_first lt).
+
+Global Instance Rtheta_Commutative_Rtheta_liftM2
+       (op: Rtheta -> Rtheta -> Rtheta)
+       `{op_mor: !Proper ((=) ==> (=) ==> (=)) op}
+       `{C: !Commutative op}
+  :
+    @Commutative (flags_m Rtheta) Rtheta_Mequiv (flags_m Rtheta) (Rtheta_liftM2 op).
+Proof.
+  intros x y.
+  unfold_Rtheta_Mequiv.
+  rewrite 2!evalWriter_lift_Rtheta_liftM2.
+  apply C.
+Qed.
+
+Global Program Instance Rtheta_val_Mabs: Abs (flags_m Rtheta) := Rtheta_liftM (Rtheta_unary abs).
+Next Obligation.
+  unfold_Rtheta_Mequiv.
+  rewrite evalWriter_Rtheta_liftM.
+  unfold le, Rtheta_Le, Rtheta_rel_first, Rtheta_unary.
+  unfold abs; crush.
+Qed.
+
+Definition Rtheta_MSZero: flags_m Rtheta := ret Rtheta_SZero.
+Definition Rtheta_MSOne: flags_m Rtheta := ret Rtheta_SOne.
+
+Lemma evalWriter_Rtheta_MSZero:
+  evalWriter Rtheta_MSZero = Rtheta_SZero.
+Proof.
+  reflexivity.
+Qed.
+
+
+
+
